exemplos/exemplos_colecoes_arrays/colecoes_arrays/ex1.dfy
@@ -1,0 +1,6 @@
+method teste()
+{
+    var a := new nat[5]; //a é do tipo array<nat>
+    a[0] := 1;
+    a[5] := 1;
+}
