exemplos/exemplos_colecoes_arrays/colecoes_arrays/ex3.dfy
@@ -1,0 +1,11 @@
+method Main()
+{
+    var a := new int[5];
+    //incializar todas posições em 0
+    forall i | 0 <= i < a.Length
+    {
+        a[i] := 0;
+    }
+    var v := a[3];
+    assert v == 0;
+}
