exemplos/exemplos_colecoes_arrays/colecoes_arrays/ex6.dfy
@@ -1,0 +1,22 @@
+method Zerar(a:array<int>)
+  //modifies a //sem essa cláusula, a verificação falha
+  ensures forall i :: 0 <= i < a.Length ==> a[i] == 0
+{
+  var i := 0;
+  while i < a.Length
+    invariant 0 <= i <= a.Length
+    invariant forall j :: 0 <= j < i ==> a[j] == 0
+  {
+    a[i] := 0;
+    i := i + 1;
+  }
+}
+
+method Main()
+{
+  var a := new int[5];
+  //incializar todas posições em 0
+  Zerar(a);
+  var v := a[3];
+  assert v == 0;
+}
