exemplos/exemplos_colecoes_arrays/colecoes_arrays/ex7.dfy
@@ -1,0 +1,24 @@
+method CriarZerado(n:nat) returns (a:array<int>)
+  requires n > 0
+  ensures a.Length == n
+  //ensures fresh(a) //sem essa cláusula, a verificação falha no método Main
+  ensures forall i :: 0 <= i < a.Length ==> a[i] == 0
+{
+  a := new int[n];
+  var i := 0;
+  while i < a.Length
+    invariant 0 <= i <= a.Length
+    invariant forall j :: 0 <= j < i ==> a[j] == 0
+  {
+    a[i] := 0;
+    i := i + 1;
+  }
+}
+
+method Main()
+{
+  var a := CriarZerado(5);
+  var v := a[3];
+  assert v == 0;
+  a[0] := 1;
+}
