exemplos/exemplos_colecoes_conjuntos/colecoes_conjuntos/ex4.dfy
@@ -1,0 +1,19 @@
+method Main()
+{
+  var a := new int[3];
+  a[0] := 1;
+  a[1] := 0;
+  a[2] := 1;
+
+  var sequencia := a[..];
+  assert sequencia == [1,0,1];
+
+  var conjunto := set num: int | num in sequencia;
+  assert conjunto == {0,1};
+
+  var multiconjunto := multiset(sequencia);
+  assert multiconjunto == multiset{0,1,1};
+
+  //quantas ocorrências de 1 no array a?
+  assert multiset(a[..])[1] == 2;
+}
