exemplos/exemplos_colecoes_conjuntos/colecoes_conjuntos/ex5.dfy
@@ -1,0 +1,22 @@
+ghost function to_seq<T>(a: array<T>, i: int) : (res: seq<T>)
+  requires 0 <= i <= a.Length
+  ensures res == a[i..]
+  reads a
+  decreases a.Length-i
+{
+  if i == a.Length
+  then []
+  else [a[i]] + to_seq(a, i + 1)
+}
+
+method Main() {
+  var a: array<int> := new int[3];
+  a[0] := 2;
+  a[1] := 3;
+  a[2] := 1;
+
+  var ms: multiset<int> := multiset(a[..]);
+  assert a[..] == to_seq(a, 0); //dica para o Dafny
+  assert ms[2] == 1;
+  assert ms[0] == 0;
+}
