exemplos/exemplos_colecoes_conjuntos/colecoes_conjuntos/ex6.dfy
@@ -1,0 +1,99 @@
+ghost predicate OrdenadoCrescente(a:array<int>)
+  reads a
+{
+    forall i,j :: 0 <= i < j < a.Length ==> a[i] <= a[j]
+}
+
+ghost predicate OrdenadoCrescenteSeq(a:seq<int>)
+{
+    forall i,j :: 0 <= i < j < |a| ==> a[i] <= a[j]
+}
+
+ghost predicate Permutacao(a:seq<int>, b:seq<int>)
+{
+    multiset(a) == multiset(b)
+}
+
+ghost predicate PontoDeQuebraEmOrdem(a:array<int>, n:int)
+  requires 0 <= n <= a.Length
+  reads a
+{
+    forall i,j :: 0 <= i < n <= j < a.Length ==> a[i] <= a[j]
+}
+
+method SelectionSort(a:array<int>)
+  modifies a
+  ensures OrdenadoCrescenteSeq(a[..])
+  ensures Permutacao(a[..], old(a[..]))
+{
+    var n := 0;
+    while n < a.Length
+      invariant 0 <= n <= a.Length
+      invariant OrdenadoCrescenteSeq(a[..n])
+      invariant Permutacao(a[..], old(a[..]))
+      invariant PontoDeQuebraEmOrdem(a,n)
+    {
+        var mindex, m := n, n+1;
+        while m < a.Length
+          invariant n <= mindex < m <= a.Length
+          invariant forall i :: n <= i < m ==> a[mindex] <= a[i]
+        {
+            if a[m] < a[mindex]
+            {
+                mindex := m;
+            }
+            m := m + 1;
+        }
+        a[n], a[mindex] := a[mindex], a[n];
+        n := n + 1;
+    }
+}
+
+method FindMinIndex(a:array<int>, s:int) returns (mindex:int)
+  requires a.Length > 0
+  requires 0 <= s < a.Length
+  ensures s <= mindex < a.Length
+  ensures forall i :: s <= i < a.Length ==> a[mindex] <= a[i]
+{
+    var index := s + 1;
+    mindex := s;
+    while index < a.Length
+      invariant s <= mindex < index <= a.Length
+      //invariant s <= index <= a.Length
+      //invariant s <= mindex < a.Length
+      invariant forall j :: s <= j < index ==> a[mindex] <= a[j]
+    {
+        if a[index] < a[mindex]
+        {
+            mindex := index;
+        }
+        index := index + 1;
+    }
+}
+
+method SelectionSortV2(a:array<int>)
+  modifies a
+  ensures OrdenadoCrescenteSeq(a[..])
+  ensures Permutacao(a[..], old(a[..]))
+{
+    var n := 0;
+    while n < a.Length
+      invariant 0 <= n <= a.Length
+      invariant OrdenadoCrescenteSeq(a[..n])
+      invariant Permutacao(a[..], old(a[..]))
+      invariant PontoDeQuebraEmOrdem(a,n)
+    {
+        var mindex := FindMinIndex(a,n);
+        a[n], a[mindex] := a[mindex], a[n];
+        n := n + 1;
+    }
+}
+
+method Main()
+{
+  var a := new int[4];
+  a[0], a[1], a[2], a[3] := 10, 1, 0, 5;
+  assert a[..] == [10,1,0,5];
+  SelectionSort(a);
+  assert a[..] == [0,1,5,10];
+}
