exemplos/exemplos_colecoes_sequences/colecoes_sequences/ex4.dfy
@@ -1,0 +1,14 @@
+// palavra contém uma string
+// remover p caracteres a partir da posição ini até fim
+method Delete(palavra:array<char>, ini:nat, fim:nat, p:nat)
+  requires fim <= palavra.Length
+  requires ini+p <= fim
+  modifies palavra
+  ensures palavra[..ini] == old(palavra[..ini])
+  ensures palavra[ini..fim-p] == old(palavra[ini+p..fim])
+{
+    forall i | 0 <= i < fim-(ini+p)
+    { 
+        palavra[ini+i] := palavra[ini+p+i];
+    }
+}
