exemplos/exercicios5_classes/exercicios_classes/exercicio2b.dfy
@@ -1,0 +1,91 @@
+class FilaNat
+{
+  //Implementação
+  var a: array<nat>
+  var cauda: nat
+  //Abstração
+  ghost var Conteudo: seq<nat>
+  ghost var Repr: set<object>
+
+  //Invariante de classe
+  ghost predicate Valid()
+    reads this, Repr
+    ensures Valid() ==> this in Repr
+  {
+    this in Repr &&
+    a in Repr &&
+    a.Length != 0 &&
+    0 <= cauda <= a.Length &&
+    Conteudo == a[0..cauda]
+  }
+
+  constructor ()
+    ensures Valid() && fresh(Repr)
+    ensures Conteudo == []
+  {
+    a := new nat[5];
+    cauda := 0;
+    Conteudo := [];
+    Repr := {this, a};
+  }
+
+  function Quantidade():nat
+    requires Valid()
+    reads Repr
+    ensures Quantidade() == |Conteudo|
+  {
+    cauda
+  }
+
+  method Enfileira(e:nat)
+    requires Valid()
+    modifies Repr
+    ensures Valid() && fresh(Repr - old(Repr))
+    ensures Conteudo == old(Conteudo) + [e]
+  {
+    if cauda == a.Length
+    {
+      var b := new nat[2 * a.Length];
+      forall i | 0 <= i < a.Length
+      {
+        b[i] := a[i];
+      }
+      Repr := Repr - {a};
+      a := b;
+      Repr := Repr + {b};
+    }
+    a[cauda] := e;
+    cauda := cauda + 1;
+    Conteudo := Conteudo + [e];
+  }
+
+  method Desenfileira() returns (e:nat)
+    requires Valid()
+    requires |Conteudo| > 0
+    modifies Repr
+    ensures Valid() && fresh(Repr - old(Repr))
+    ensures e == old(Conteudo[0])
+    ensures Conteudo == old(Conteudo)[1..]
+  {
+    e := a[0];
+    cauda := cauda - 1;
+    forall i | 0 <= i < cauda
+    {
+      a[i] := a[i+1];
+    }
+    Conteudo := a[0..cauda];
+  }
+}
+
+method Main()
+{
+  var fila := new FilaNat();
+  fila.Enfileira(1);
+  fila.Enfileira(2);
+  assert fila.Conteudo == [1,2];
+  var q := fila.Quantidade();
+  assert q == 2;
+  var e := fila.Desenfileira();
+  assert e == 1;
+  assert fila.Conteudo == [2];
+}
